Switch to sets for collecting preds

state/experiments/ComputationalView.fst
@@ -36,7 +36,7 @@ let rec freePure_to_pureId #a (m:freePure a) (wp:pure_wp a) (post:a -> Type0) :
     freePure_to_pureId (k ()) (freePure_theta (k())) post
 
 assume val state_t:Type0
-assume val state_rel : state_t -> state_t -> Type0
+assume val state_rel : FStar.Preorder.preorder state_t
 
 noeq
 type freeState (a:Type) =
@@ -60,7 +60,7 @@ let rec freeState_theta (m:freeState 'a) : state_wp 'a =
 let state a = state_t -> a * state_t
 
 let rec freeState_to_state #a (m:freeState a) (wp:(state_wp a){freeState_theta m `state_wp_stronger` wp}) (post:(a -> state_t -> Type0)) (s0:state_t{wp post s0}) :
-  Tot (r:(a * state_t){post (fst r) (snd r)}) =
+  Tot (r:(a * state_t){post (fst r) (snd r) /\ s0 `state_rel` (snd r)}) =
   match m with
   | ReturnST x -> (x, s0)
   | GetST k ->  freeState_to_state (k s0) (freeState_theta (k s0)) post s0
@@ -108,8 +108,10 @@ let rec freeMST_to_state #a (m:freeMST a) (wp:(state_wp a){freeMST_theta witness
 type stable_pred =
   pred:(state_t -> Type0){forall h0 h1. pred h0 /\ h0 `state_rel` h1 ==> pred h1}
 
+module S = FStar.TSet
+
 type statepreds =
-  sp:(state_t * list stable_pred){forall (pred:stable_pred). pred `List.Tot.memP` (snd sp) ==> pred (fst sp)}
+  sp:(state_t * S.set stable_pred){forall (pred:stable_pred). pred `S.mem` (snd sp) ==> pred (fst sp)}
   
 val witnessed' : (state_t -> Type0) -> Type0
 let witnessed' pred = True // i don't have access to the heap
@@ -125,13 +127,13 @@ let rec freeMST_to_state' #a (m:freeMST a) (wp:(state_wp a){freeMST_theta witnes
     assert (witnessed' pred ==> freeMST_theta witnessed' (k ()) post (fst s0));
     assume (forall h0 h1. pred h0 /\ h0 `state_rel` h1 ==> pred h1); // one has to strengthen the type of witness/recall
     assert (witnessed' pred);
-    let lp = snd s0 @ [pred] in
-    assume (forall (pred:stable_pred). pred `List.Tot.memP` lp ==> pred (fst s0)); // probably easy to prove by induction;
+    let lp = S.union (snd s0) (S.singleton pred) in
+    assume (forall (pred:stable_pred). pred `S.mem` lp ==> pred (fst s0)); // probably easy to prove by induction;
     freeMST_to_state' (k ()) (freeMST_theta witnessed' (k ())) post (fst s0, lp)
   | RecallMST pred k -> 
     assert (witnessed' pred);
     assume (forall h0 h1. pred h0 /\ h0 `state_rel` h1 ==> pred h1); // one has to strengthen the type of witness/recall
-    assume (pred `List.Tot.memP` (snd s0));
+    assume (pred `S.mem` (snd s0));
     assert (pred (fst s0)); (** 
       CA: i need to know here that pred is in the list of predicates.
       In pulse, they have an index that tells them that the predicate is contained **)
